test-suite/iso/squiggle5StrongIso.v
@@ -20,40 +20,41 @@ Require Import ReflParam.Trecord.
 Require Import ReflParam.unusedVar.
 Declare ML Module "myplug".
 Section Test.
-Variables (A A₂ : Set)
-(Ra : A -> A₂ -> Prop)
-(pta : TotalHeteroRel Ra)
-(B B₂ : Set)
-(Rb : B -> B₂ -> Prop)
-(ptb : TotalHeteroRel Rb)
-(poa : oneToOne Ra)
+Variables 
+(Tm Tm₂ : Set)
+(Tmᵣ : Tm -> Tm₂ -> Prop)
+(TmᵣTot : TotalHeteroRel Tmᵣ)
+(BTm BTm₂ : Set)
+(BTmᵣ : BTm -> BTm₂ -> Prop)
+(BTmᵣTot : TotalHeteroRel BTmᵣ)
+(TmᵣOne : oneToOne Tmᵣ)
 .
 Check(
-fun (pob : oneToOne Rb) =>
-let A_R := (@Build_GoodRel allProps _ _ Ra pta poa) in
-let B_R := (@Build_GoodRel allProps _ _ Rb ptb pob) in
+fun (BTmᵣOne : oneToOne BTmᵣ) =>
+let A_R := (@Build_GoodRel allProps _ _ Tmᵣ TmᵣTot TmᵣOne) in
+let B_R := (@Build_GoodRel allProps _ _ BTmᵣ BTmᵣTot BTmᵣOne) in
 Top_squiggle5_obseq_pmtcty_RR _ _ A_R _ _ B_R
 ).
 
-Time Detect (
-fun (pob : oneToOne Rb) =>
-let A_R := (@Build_GoodRel allProps _ _ Ra pta poa) in
-let B_R := (@Build_GoodRel allProps _ _ Rb ptb pob) in
-Top_squiggle5_obsEq_pmtcty_RR _ _ A_R _ _ B_R
+Time Detect(
+fun (BTmᵣOne : oneToOne BTmᵣ) =>
+let A_R := (@Build_GoodRel allProps _ _ Tmᵣ TmᵣTot TmᵣOne) in
+let B_R := (@Build_GoodRel allProps _ _ BTmᵣ BTmᵣTot BTmᵣOne) in
+Top_squiggle5_obseq_pmtcty_RR _ _ A_R _ _ B_R
 ).
 
 Time 
 ReduceAwayLamVar sthm := (
-fun (pob : oneToOne Rb) =>
-let A_R := (@Build_GoodRel allProps _ _ Ra pta poa) in
-let B_R := (@Build_GoodRel allProps _ _ Rb ptb pob) in
+fun (BTmᵣOne : oneToOne BTmᵣ) =>
+let A_R := (@Build_GoodRel allProps _ _ Tmᵣ TmᵣTot TmᵣOne) in
+let B_R := (@Build_GoodRel allProps _ _ BTmᵣ BTmᵣTot BTmᵣOne) in
 Top_squiggle5_obseq_pmtcty_RR _ _ A_R _ _ B_R
 ).
 
 Check sthm.
-Lemma testDefn (pob : oneToOne Rb):
-let A_R := (@Build_GoodRel allProps _ _ Ra pta poa) in
-let B_R := (@Build_GoodRel allProps _ _ Rb ptb pob) in
+Lemma testDefn (BTmᵣOne : oneToOne BTmᵣ):
+let A_R := (@Build_GoodRel allProps _ _ Tmᵣ TmᵣTot TmᵣOne) in
+let B_R := (@Build_GoodRel allProps _ _ BTmᵣ BTmᵣTot BTmᵣOne) in
 JMeq 
   (Top_squiggle5_obseq_pmtcty_RR _ _ A_R _ _ B_R)
   sthm.
@@ -64,21 +65,21 @@ Qed.
 End Test.
 
 Section Test2.
-Variables (A A₂ : Set)
-(Ra : A -> A₂ -> Prop)
-(pta : TotalHeteroRel Ra)
-(B B₂ : Set)
-(Rb : B -> B₂ -> Prop)
-(ptb : TotalHeteroRel Rb).
+Variables 
+(Tm Tm₂ : Set)
+(Tmᵣ : Tm -> Tm₂ -> Prop)
+(TmᵣTot : TotalHeteroRel Tmᵣ)
+(BTm BTm₂ : Set)
+(BTmᵣ : BTm -> BTm₂ -> Prop).
 
 Check (
-fun (poa : oneToOne Ra) =>
-@sthm _ _ Ra pta _ _ Rb poa
+fun (poa : oneToOne Tmᵣ) =>
+@sthm _ _ Tmᵣ TmᵣTot _ _ BTmᵣ poa
 ).
 Time Detect
 (
-fun (poa : oneToOne Ra) =>
-sthm _ _ Ra pta _ _ Rb poa
+fun (poa : oneToOne Tmᵣ) =>
+@sthm _ _ Tmᵣ TmᵣTot _ _ BTmᵣ poa
 ).
 (*The first argument may be omitted. The reduced term is:...
 Finished transaction in 1.694 secs (1.447u,0.011s) (successful)
@@ -86,8 +87,8 @@ Finished transaction in 1.694 secs (1.447u,0.011s) (successful)
 
 Time  ReduceAwayLamVar obseqStrongIso := 
 (
-fun (poa : oneToOne Ra) =>
-sthm A A₂ Ra pta B B₂ Rb poa
+fun (poa : oneToOne Tmᵣ) =>
+@sthm _ _ Tmᵣ TmᵣTot _ _ BTmᵣ poa
 ).
 
 (*
@@ -106,6 +107,62 @@ Abort. (* Qed works, but this using Abort because this lemma should not be used,
 
 
 Check obseqStrongIso.
+
+Check Top_squiggle5_TmKind_pmtcty_RR0.
+
+(* folding definitions and alpha renaming for readability *)
+Definition obseqStrongIsoType :=
+forall 
+  (Tm Tm₂ : Set) (Tmᵣ : Tm -> Tm₂ -> Prop)
+  (Tmᵣtot: TotalHeteroRel Tmᵣ)
+  (BTm BTm₂ : Set) (BTmᵣ : BTm -> BTm₂ -> Prop)
+  (applyBtm : BTm -> Tm -> Tm) (applyBtm₂ : BTm₂ -> Tm₂ -> Tm₂)
+  (applyBtmᵣ : forall (b : BTm) (b₂ : BTm₂) (bᵣ: BTmᵣ b b₂) 
+    (a : Tm) (a₂ : Tm₂) (aᵣ : Tmᵣ a a₂), Tmᵣ (applyBtm b a) (applyBtm₂ b₂ a₂))
+  (tmKind : Tm -> TmKind Tm BTm)
+  (tmKind₂ : Tm₂ -> TmKind Tm₂ BTm₂)
+  (tmKindᵣ : forall (a : Tm) (a₂ : Tm₂)
+        (aᵣ: Tmᵣ a a₂),
+        Top_squiggle5_TmKind_pmtcty_RR0 Tm Tm₂ Tmᵣ BTm BTm₂ BTmᵣ (tmKind a)
+          (tmKind₂ a₂))
+  (tl : Tm) (tl₂ : Tm₂)
+  (tlᵣ: Tmᵣ tl tl₂)
+  (tr : Tm) (tr₂ : Tm₂)
+  (trᵣ: Tmᵣ tr tr₂),
+     BestRel (obseq Tm BTm applyBtm tmKind tl tr)
+             (obseq Tm₂ BTm₂ applyBtm₂ tmKind₂ tl₂ tr₂).
+
+Goal JMeq obseqStrongIsoType ltac:(let T:=type of obseqStrongIso in exact T).
+reflexivity.
+Qed.
+
+Definition obseqWeakIsoType :=
+(forall (Tm Tm₂ : Set) (Tm_R : BestRel Tm Tm₂) (BTm BTm₂ : Set)
+   (BTm_R : BestRel BTm BTm₂) (applyBtm : BTm -> Tm -> Tm)
+   (applyBtm₂ : BTm₂ -> Tm₂ -> Tm₂),
+ (forall (a1 : BTm) (a2 : BTm₂),
+  BestR BTm_R a1 a2 ->
+  forall (a3 : Tm) (a4 : Tm₂),
+  BestR Tm_R a3 a4 -> BestR Tm_R (applyBtm a1 a3) (applyBtm₂ a2 a4)) ->
+ forall (tmKind : Tm -> TmKind Tm BTm) (tmKind₂ : Tm₂ -> TmKind Tm₂ BTm₂),
+ (forall (a1 : Tm) (a2 : Tm₂),
+  BestR Tm_R a1 a2 ->
+  Top_squiggle5_TmKind_pmtcty_RR0 Tm Tm₂ (BestR Tm_R) BTm BTm₂ (BestR BTm_R)
+    (tmKind a1) (tmKind₂ a2)) ->
+ forall (tl : Tm) (tl₂ : Tm₂),
+ BestR Tm_R tl tl₂ ->
+ forall (tr : Tm) (tr₂ : Tm₂),
+ BestR Tm_R tr tr₂ ->
+ BestRel (forall a : nat, obsEq Tm BTm applyBtm tmKind a tl tr)
+   (forall a : nat, obsEq Tm₂ BTm₂ applyBtm₂ tmKind₂ a tl₂ tr₂)).
+
+Goal False.
+let T:=type of Top_squiggle5_obseq_pmtcty_RR in let t:= eval simpl in T in idtac t.
+Abort.
+
+Goal JMeq obseqWeakIsoType ltac:(let T:=type of Top_squiggle5_obseq_pmtcty_RR in exact T).
+reflexivity.
+Qed.
 (*
 Lemma dependsOnlyOnTotdivergesIff  : existsAOneFreeImpl
   (Top_squiggle2_divergesIff_pmtcty_RR).
